Numeral adventures.

garbage/Numeral.v
@@ -1,25 +1,38 @@
-From Coq Require Import NArith List Decimal Ascii String.
+From Coq Require Import Ascii Decimal List NArith String.
 
-Import ListNotations.
+Module StringNotations.
+
+Notation "x '::' xs" := (String x xs) : string_scope.
+Notation "'[' ']'" := EmptyString : string_scope.
+Notation "'[' x ']'" := (String x EmptyString) : string_scope.
+Notation "'[' x ';' y ';' .. ';' z ']'" :=
+  (String x (String y .. (String z EmptyString) ..)) : string_scope.
+
+End StringNotations.
+
+Import StringNotations.
 
 Fixpoint string_of_uint (n : uint) : string :=
   match n with
-  | Nil => ""%string
-  | D0 p => String "0"%char (string_of_uint p)
-  | D1 p => String "1"%char (string_of_uint p)
-  | D2 p => String "2"%char (string_of_uint p)
-  | D3 p => String "3"%char (string_of_uint p)
-  | D4 p => String "4"%char (string_of_uint p)
-  | D5 p => String "5"%char (string_of_uint p)
-  | D6 p => String "6"%char (string_of_uint p)
-  | D7 p => String "7"%char (string_of_uint p)
-  | D8 p => String "8"%char (string_of_uint p)
-  | D9 p => String "9"%char (string_of_uint p)
+  | Nil => ""
+  | D0 p => "0" :: string_of_uint p
+  | D1 p => "1" :: string_of_uint p
+  | D2 p => "2" :: string_of_uint p
+  | D3 p => "3" :: string_of_uint p
+  | D4 p => "4" :: string_of_uint p
+  | D5 p => "5" :: string_of_uint p
+  | D6 p => "6" :: string_of_uint p
+  | D7 p => "7" :: string_of_uint p
+  | D8 p => "8" :: string_of_uint p
+  | D9 p => "9" :: string_of_uint p
   end.
 
 Section Natural.
 
-Import N.
+Import ListNotations N.
+
+Definition string_of_N (n : N) : string :=
+  string_of_uint (to_uint n).
 
 Open Scope N_scope.
 
@@ -28,9 +41,6 @@ Fixpoint N_compute (ns : list N) : N :=
   | [] => 0
   | p :: ps => p + N_compute ps
   end.
-
-Definition string_of_N (n : N) : string :=
-  string_of_uint (to_uint n).
 
 Fixpoint N_format (ns : list N) : string :=
   match ns with
@@ -45,17 +55,14 @@ End Natural.
 
 Section Positive.
 
-Import Pos.
+Import ListNotations Pos.
 
 Open Scope positive_scope.
 
-Reserved Notation "'double'" (at level 0, no associativity).
-Notation "'double'" := xO (only parsing) : positive_scope.
-
 Fixpoint positive_powers_of_two (n : positive) : list positive :=
   match n with
-  | p ~ 1 => 1 :: map double (positive_powers_of_two p)
-  | p ~ 0 => map double (positive_powers_of_two p)
+  | p ~ 1 => 1 :: map xO (positive_powers_of_two p)
+  | p ~ 0 => map xO (positive_powers_of_two p)
   | 1 => [1]
   end.
 
@@ -63,16 +70,20 @@ End Positive.
 
 Section Natural.
 
-Import N.
+Import ListNotations N.
 
-Open Scope N_scope.
 Open Scope string_scope.
+Open Scope list_scope.
+Open Scope N_scope.
 
 Definition N_powers_of_two (n : N) : list N :=
   match n with
   | 0 => []
   | pos p => map pos (positive_powers_of_two p)
   end.
+
+Compute map (fun n : N => N_compute (N_powers_of_two n))
+  (map of_nat (seq 0 16)).
 
 Compute map (fun n : N => N_format (N_powers_of_two n))
   (map of_nat (seq 0 16)).
@@ -82,7 +93,7 @@ Lemma N_compute_map_double : forall ns : list N,
 Proof.
   intros ns. induction ns as [| p ps IH].
   - reflexivity.
-  - cbn. rewrite IH. rewrite double_add. reflexivity. Qed.
+  - cbn [map N_compute]. rewrite IH. rewrite double_add. reflexivity. Qed.
 
 Theorem N_powers_of_two_valid : forall n : N,
   N_compute (N_powers_of_two n) = n.
@@ -90,49 +101,39 @@ Proof.
   intros n. destruct n as [| p].
   - reflexivity.
   - cbv [N_powers_of_two]. induction p as [q IH | q IH |].
-    + cbn. rewrite map_map.
+    + cbn [positive_powers_of_two map N_compute]. rewrite map_map.
       replace (fun x : positive => pos x ~ 0) with
-        (fun x : positive => N.double (pos x)) by reflexivity.
+        (fun x : positive => double (pos x)) by reflexivity.
       rewrite <- map_map. rewrite N_compute_map_double.
       rewrite IH. reflexivity.
-    + cbn. rewrite map_map.
+    + cbn [positive_powers_of_two]. rewrite map_map.
       replace (fun x : positive => pos x ~ 0) with
-        (fun x : positive => N.double (pos x)) by reflexivity.
+        (fun x : positive => double (pos x)) by reflexivity.
       rewrite <- map_map. rewrite N_compute_map_double.
       rewrite IH. reflexivity.
     + reflexivity. Qed.
 
 End Natural.
 
-(** Add a power of two and a residue. *)
-
-Section Positive.
-
-Import Pos.
-
-Open Scope positive_scope.
-
-Reserved Notation "x '/' '2'" (at level 40, left associativity).
-Notation "x '/' '2'" := (Pos.div2 x) : positive_scope.
-
-Definition positive_power_and_residue (n : positive) : list positive :=
-  if n =? 1 then [1] else let p : positive := size n - 1 in
-  if n =? 2 ^ p then [n / 2; n / 2] else [n - 2 ^ p; 2 ^ p].
-
-End Positive.
+(** Add a power of two and its residue. *)
 
 Section Natural.
 
-Import N.
+Import ListNotations N.
 
-Open Scope N_scope.
 Open Scope string_scope.
+Open Scope list_scope.
+Open Scope N_scope.
 
 Definition N_power_and_residue (n : N) : list N :=
-  match n with
-  | 0 => []
-  | pos p => map pos (positive_power_and_residue p)
-  end.
+  if n =? 0 then [] else
+  if n =? 1 then [1] else
+  let p : N := log2 n in
+  if n =? 2 ^ p then [n / 2; n / 2] else
+  [n - 2 ^ p; 2 ^ p].
+
+Compute map (fun n : N => N_compute (N_power_and_residue n))
+  (map of_nat (seq 0 16)).
 
 Compute map (fun n : N => N_format (N_power_and_residue n))
   (map of_nat (seq 0 16)).
@@ -140,19 +141,21 @@ Compute map (fun n : N => N_format (N_power_and_residue n))
 Theorem N_power_and_residue_valid : forall n : N,
   N_compute (N_power_and_residue n) = n.
 Proof.
-  intros n. destruct n as [| p].
-  - reflexivity.
-  - cbv [N_power_and_residue positive_power_and_residue].
-    destruct (Pos.eqb_spec p 1)%positive as [H | H].
-    + rewrite H. reflexivity.
-    + destruct (Pos.eqb_spec p (2 ^ (Pos.size p - 1)))%positive as [H' | H'].
-      * cbn. f_equal. destruct p as [q | q |]. all: cbn in *.
-        -- admit.
-        -- rewrite Pos.add_diag. reflexivity.
-        -- exfalso. apply H. reflexivity.
-      * cbn. f_equal. destruct p as [q | q |]. all: cbn in *.
-        -- admit.
-        -- admit.
-        -- exfalso. apply H. reflexivity. Admitted.
+  intros n. cbv [N_power_and_residue].
+  destruct (eqb_spec n 0) as [H0 | H0].
+  - rewrite H0. reflexivity.
+  - destruct (eqb_spec n 1) as [H1 | H1].
+    + rewrite H1. reflexivity.
+    + destruct (eqb_spec n (2 ^ log2 n)) as [H2 | H2].
+      * cbv [N_compute]. ring_simplify.
+        destruct (log2 n) as [| p _] using peano_ind.
+        -- exfalso. apply H1. apply H2.
+        -- pose proof (neq_succ_0 1) as H.
+          symmetry. rewrite (div_exact n 2 H). rewrite (mod_divides n 2 H).
+          exists (2 ^ p). rewrite <- pow_succ_r'. apply H2.
+      * cbv [N_compute]. ring_simplify.
+        rewrite (sub_add (2 ^ log2 n) n).
+        -- reflexivity.
+        -- apply log2_spec. rewrite <- (neq_0_lt_0 n). apply H0. Qed.
 
 End Natural.
