prototype/Offers/FieldConstants.v
@@ -3,19 +3,85 @@ From Maniunfold.Has Require Export
 From Maniunfold.ShouldHave Require Export
   FieldNotations.
 
+(** Semirings only come with zero and one out of the box,
+    so we have to construct all the other natural numbers
+    from repeated additions and multiplications.
+    The optimal way to do this is quite complicated,
+    as demonstrated in OEIS sequence A005245,
+    but we can make the job more manageable
+    by limiting ourselves to just addition. *)
+
+(** The following definitions produce
+    the natural numbers using the simplest suboptimal reduction tree. *)
+
+Section Context.
+
+Context {A : Type} {has_add : HasAdd A} {has_zero : HasZero A}
+  {has_one : HasOne A}.
+
+Fixpoint of_nat (n : nat) : A :=
+  match n with
+  | O => 0
+  | S p => 1 + of_nat p
+  end.
+
+End Context.
+
+(** The following definitions produce
+    the natural numbers using one of the optimal reduction trees. *)
+
+(** TODO Clean up the termination proof. *)
+
+Require Import List Program Recdef Omega PeanoNat.
+
+Section Context.
+
+Import ListNotations Nat.
+
+Context {A : Type} {has_add : HasAdd A} {has_zero : HasZero A}
+  {has_one : HasOne A}.
+
+Function of_nat' (n : nat) {measure id n} : A :=
+  if n =? 0 then 0 else
+  if n =? 1 then 1 else
+  let p : nat := log2 n in
+  if n =? 2 ^ p then of_nat' (n / 2) + of_nat' (n / 2) else
+  of_nat' (n - 2 ^ p) + of_nat' (2 ^ p).
+Proof.
+  { intros n H0 H1 H2.
+    apply eqb_neq in H0. apply eqb_neq in H1. apply eqb_eq in H2. cbv [id].
+    rewrite H2.
+    pose proof (neq_succ_0 1) as H.
+    epose proof log2_spec n _ as H'. rewrite pow_succ_r' in H'.
+    eapply le_lt_trans.
+      apply div_le_mono. apply H. apply (proj1 H').
+      apply (div_lt_upper_bound _ _ _ H). apply H'. }
+  { intros n H0 H1 H2.
+    apply eqb_neq in H0. apply eqb_neq in H1. apply eqb_neq in H2. cbv [id].
+    pose proof (neq_succ_0 1) as H.
+    epose proof log2_spec n _ as H'. rewrite pow_succ_r' in H'.
+    rewrite le_neq. split.
+      apply H'.
+      apply neq_sym. apply H2. }
+  { intros n H0 H1 H2.
+    apply eqb_neq in H0. apply eqb_neq in H1. apply eqb_neq in H2. cbv [id].
+    pose proof (neq_succ_0 1) as H.
+    epose proof log2_spec n _ as H'. rewrite pow_succ_r' in H'.
+    apply sub_lt.
+      apply H'. epose proof mul_lt_mono_pos_l 2 0 (2 ^ log2 n) _.
+      apply H3. eapply lt_trans.
+      apply neq_0_lt. apply neq_sym. apply H0.
+      apply H'. }
+Unshelve. all: omega. Defined.
+
+End Context.
+
+(** The following definitions produce
+    the first few natural numbers as special cases. *)
+
 Section Context.
 
 Context {A : Type} {has_add : HasAdd A} {has_one : HasOne A}.
-
-(** Semirings only come with zero and one,
-    but we can construct any other natural number
-    by adding or multiplying them together.
-    The optimal way to do this is quite complicated,
-    as demonstrated in OEIS sequence A005245.
-    However, we can make the construction more manageable
-    by limiting ourselves to just addition.
-    The following definitions produce an optimal reduction tree (one of many)
-    for constructing the first few natural numbers from additions. *)
 
 Definition two : A := one + one.
 Definition three : A := two + one.
